feat: allow users to mark definitions with `[simp]`
cc @JasonGross @Kha

src/Lean/Meta/Tactic/Simp/Main.lean
@@ -58,7 +58,7 @@ private def reduceProjFn? (e : Expr) : SimpM (Option Expr) := do
     | none => return none
     | some projInfo =>
       if projInfo.fromClass then
-        if (← read).toUnfold.contains cinfo.name then
+        if (← read).simpLemmas.isDeclToUnfold cinfo.name then
           -- We only unfold class projections when the user explicitly requested them to be unfolded.
           -- Recall that `unfoldDefinition?` has support for unfolding this kind of projection.
           withReducibleAndInstances <| unfoldDefinition? e
@@ -88,7 +88,7 @@ private def unfold? (e : Expr) : SimpM (Option Expr) := do
   let fName := f.constName!
   if (← isProjectionFn fName) then
     return none -- should be reduced by `reduceProjFn?`
-  if (← read).toUnfold.contains e.getAppFn.constName! then
+  if (← read).simpLemmas.isDeclToUnfold e.getAppFn.constName! then
     withDefault <| unfoldDefinition? e
   else
     return none
