tests/lean/run/simpDefToUnfold.lean
@@ -1,0 +1,20 @@
+@[simp] def f (x : Nat) := x + 1
+
+@[simp] def g (x : Nat) := id x
+
+def h (x : Nat) := g (g x)
+
+namespace Extra
+  attribute [scoped simp] h
+end Extra
+
+theorem ex1 : f (g (h x)) = x + 1 := by
+  simp -- did not unfold h
+  simp [h]
+
+theorem ex2 : f (g (h x)) = x + 1 := by
+  open Extra in simp -- unfold f,g,h
+
+theorem ex3 : f (g x) = x + 1 := by
+  simp [-f] -- did not unfold f
+  simp
